Updating to coq 8.9 andf recent Compcert (does not compile, See the last commit in this series)

compcert_new/backend/Linear.v
@@ -287,7 +287,7 @@ Inductive step: state -> trace -> state -> Prop :=
       forall s ef args res rs1 rs2 m t m',
       args = map (fun p => Locmap.getpair p rs1) (loc_arguments (ef_sig ef)) ->
       external_call ef ge args m t res m' ->
-      rs2 = Locmap.setpair (loc_result (ef_sig ef)) res rs1 ->
+      rs2 = Locmap.setpair (loc_result (ef_sig ef)) res (undef_caller_save_regs rs1) ->
       step (Callstate s (External ef) rs1 m)
          t (Returnstate s rs2 m')
   | exec_return:
@@ -317,7 +317,6 @@ Inductive entry_point (p: program): mem -> state -> val -> list val -> Prop :=
       Genv.find_funct_ptr ge b = Some f ->
       Val.has_type_list args (sig_args (funsig f)) ->
       Genv.find_funct_ptr ge b0 = Some (Internal f0) ->
-      tailcall_possible (fn_sig f0) ->
 (*      size_arguments (funsig f) <= Z.max (max_over_instrs outgoing_space) (max_over_slots_of_funct outgoing_slot) ->*)
       Mem.alloc m0 0 (fn_stacksize f0) = (m1, stk) ->
       let ls := build_ls_from_arguments (funsig f) args in
