compcert_new/common/Events.v
@@ -1323,7 +1323,6 @@ Proof.
   exists v1; constructor; auto.
 Qed.
 
-
 (* Lemma volatile_load_trivial_inject:
   forall {ge chunk m b ofs t vres},
     volatile_load ge chunk m b ofs t vres ->
